changed CompileModule.v back

platform/cito/CompileModule.v
@@ -5,37 +5,70 @@ Require Import GoodFunc GoodOptimizer.
 
 Set Implicit Arguments.
 
-Definition GoodFunc := { f | GoodFunc.GoodFunc f }.
+Definition NameNotInImports name imports := 
+  fold_left
+    (fun (b : bool) (p : string * string * assert) =>
+       let '(m, _, _) := p in
+       (b || (if string_dec m name then true else false))%bool)
+    imports false = false.
 
-Require Import Semantics.
-Record GoodModule :=
-  {
-    Name : string;
-    Imports : LabelMap.t Callee;
-    Funcs : list GoodFunc
-  }.
-    
+Definition NoDupFuncNames mod_name funcs :=
+  match
+    fold_left
+      (fun (mOpt : option (LabelMap.t unit))
+           (p : string * assert *
+                (forall imports : LabelMap.t assert,
+                   importsGlobal imports -> cmd imports mod_name)) =>
+         let '(modl, _, _) := p in
+         match mOpt with
+           | Some m =>
+             let k := (modl, Local 0) in
+             if LabelMap.mem (elt:=unit) k m
+             then None
+             else Some (LabelMap.add k tt m)
+           | None => None
+         end) funcs (Some (LabelMap.empty unit))
+  with
+    | Some _ => True
+    | None => False
+  end.
+
 Section TopSection.
 
-  Variable module : GoodModule.
+  Variable module : CitoModule.
+
+  Require Import CompileFuncImpl.
+  Record GoodModule module := 
+    {
+      NoDupFuncNames_ : NoDup (map Name (Functions module));
+      GoodFuncs : List.Forall GoodFunc (Functions module)
+    }.
+
+  Hypothesis good_module : GoodModule module.
 
   Require Import StructuredModule.
-  Definition imports : list import.
-    admit.
-  Qed.
+  Definition imports : list import := nil.
 
   Variable optimizer : Optimizer.
 
   Hypothesis good_optimizer : GoodOptimizer optimizer.
 
-  Definition compile_func' f (good_func : GoodFunc.GoodFunc f) := CompileFunc.compile (Name module) good_func good_optimizer.
+  Definition to_prod_list : forall A P (ls : list A), List.Forall P ls -> list { x | P x }.
+    induction ls.
+    econstructor 1.
+    econstructor 2.
+    econstructor; inversion H; subst; eauto.
+    eapply IHls; inversion H; subst; eauto.
+  Defined.
 
-  Definition compile_func (p : GoodFunc) :=
+  Definition compile_func' f (good_func : GoodFunc f) := CompileFunc.compile (ModuleName module) good_func good_optimizer.
+
+  Definition compile_func (p : { f | GoodFunc f }) :=
     match p with
       | exist _ good_func => compile_func' good_func
     end.
 
-  Definition compiled_funcs := map compile_func (Funcs module).
+  Definition compiled_funcs := map compile_func (to_prod_list (GoodFuncs good_module)).
 
   Require Import Structured.
   Require Import Wrap.
@@ -45,10 +78,18 @@ Section TopSection.
 
   Definition compile := StructuredModule.bmodule_ imports compiled_funcs.
 
+  Lemma module_name_not_in_imports : NameNotInImports (ModuleName module) imports.
+    unfold NameNotInImports; eauto.
+  Qed.
+
+  Lemma no_dup_func_names : NoDupFuncNames compiled_funcs.
+    admit.
+  Qed.
+
   Theorem compileOk : XCAP.moduleOk compile.
     eapply bmoduleOk.
-    admit.
-    admit.
+    eapply module_name_not_in_imports.
+    eapply no_dup_func_names.
     eapply good_vcs.
   Qed.
 
